Bytes.v: Added bcombine_list: list byte -> bytes and proved some correctness theorems about it.
AByteFile.v: Defined many admitted functions and added some more helper functions. rep is working but read_ok is broken again. Implicit parameter inference problem.

src/Bytes.v
@@ -2,6 +2,8 @@ Require Import Word.
 Require Import Arith.
 Require Import Eqdep_dec.
 Require Import AsyncDisk.
+Require Import List ListUtils.
+Require Import Omega.
 
 Set Implicit Arguments.
 
@@ -10,11 +12,16 @@ Definition bytes n := word (n * 8).
 
 Definition word2bytes nbits nbytes (H : nbits = nbytes * 8) (w : word nbits) : bytes nbytes :=
   eq_rect nbits word w (nbytes*8) H.
+  
+Definition byte0 := natToWord 8 0.
+Definition bytes0 := (word2bytes 0 eq_refl WO).
+  
+Definition byte2bytes (b: byte) : bytes 1 := word2bytes 1 eq_refl b.
 
 Definition bcombine (sz1 : nat) (bs1 : bytes sz1) (sz2 : nat) (bs2 : bytes sz2) : bytes (sz1 + sz2).
   unfold bytes in *.
   rewrite Nat.mul_add_distr_r in *.
-  exact (combine bs1 bs2).
+  exact (Word.combine bs1 bs2).
 Defined.
 
 Definition bsplit1 (sz1 sz2 : nat) (bs : bytes (sz1 + sz2)) : bytes sz1.
@@ -35,7 +42,7 @@ Definition bsplit1_dep sz sz1 sz2 (v : bytes sz) (H : sz = sz1 + sz2) : bytes sz
 Definition bsplit2_dep sz sz1 sz2 (v : bytes sz) (H : sz = sz1 + sz2) : bytes sz2 :=
   bsplit2 sz1 sz2 (eq_rect sz bytes v _ H).
 
-Hint Rewrite combine_split : bytehints.
+Hint Rewrite Word.combine_split : bytehints.
 Hint Rewrite split1_combine : bytehints.
 Hint Rewrite split2_combine : bytehints.
 Hint Rewrite eq_rect_nat_double : bytehints.
@@ -73,6 +80,37 @@ Program Fixpoint bsplit_list sz (w: bytes sz) : list byte :=
     | O => nil
     | S sz => bsplit1_dep 1 sz w _ :: bsplit_list (bsplit2_dep 1 sz w _)
     end.
+
+Program Fixpoint bcombine_list (l: list byte): bytes (length l) :=
+    match l with
+     | nil => bytes0
+     | h::l' => bcombine (byte2bytes h) (bcombine_list l')
+    end.
+
+Theorem list2bytes2list: forall (l: list byte), bsplit_list (bcombine_list l) = l.
+Proof.
+  induction l.
+  unfold bsplit_list, bcombine_list. reflexivity.
+  simpl; unfold bsplit2_dep.
+  simpl; rewrite bsplit2_bcombine.
+  rewrite IHl.
+  unfold bsplit1_dep.
+  simpl; rewrite bsplit1_bcombine.
+  unfold byte2bytes.
+  reflexivity.
+Qed.
+
+Lemma split_len_eq: forall sz (b: bytes sz), length (bsplit_list b) = sz.
+Proof.
+  intros; unfold bsplit_list.
+  induction sz. 
+  reflexivity. 
+  simpl; rewrite IHsz. 
+  reflexivity.
+Qed.
+
+Theorem bytes2list2bytes2list: forall sz (b: bytes sz), bsplit_list (bcombine_list (bsplit_list b)) = bsplit_list b.
+Proof. intros; rewrite list2bytes2list. reflexivity. Qed.
 
 Notation "'valubytes'" := (Valulen.valubytes).
 Notation "'valubytes_is'" := (Valulen.valubytes_is).
